{
 "cells": [
  {
   "cell_type": "markdown",
   "id": "higher-bulgarian",
   "metadata": {},
   "source": [
    "### Problem 1 (10 Points)\n",
    "\n",
    "Sketch graphically the problem \n",
    "\n",
    "$$\n",
    "\\begin{aligned}\n",
    "\\min_{x_1,x_2} & \\quad f({\\bf x})=(x_1+1)^2+(x_2-2)^2\\\\\n",
    "{\\text{subject to }} & \\quad g_1 = x_1-2\\leq 0,{\\quad} g_3 = -x_1\\leq 0,\\\\\n",
    "& \\quad g_2 = x_2-1\\leq 0, {\\quad} g_4 = -x_2\\leq 0.\n",
    "\\end{aligned}\n",
    "$$\n",
    "\n",
    "Find the optimum graphically. Determine directions of feasible descent at the corner points of the feasible domain. Show the gradient directions of $f$ and $g_i$s at these points. Verify graphical results analytically using the KKT conditions.\n",
    "\n",
    "### Solution\n",
    "\n",
    "![Alt text](./img/prob50201.png)\n",
    " \n",
    "\n",
    "Graphic solution shows the optimum at ${\\bf x}_*=(0,1)^T$ and $f_*=2$.\n",
    "\n",
    "![Alt text](./img/prob50202.png)\n",
    "\n",
    "At (0,0): The angle marked includes the directions of feasible direction.\n",
    "\n",
    "![Alt text](./img/prob50203.png)\n",
    "\n",
    "At (2,0): The angle marked includes the directions of feasible direction.\n",
    "\n",
    "![Alt text](./img/prob50204.png)\n",
    "\n",
    "At (2,1): The angle marked includes the directions of feasible direction.\n",
    "\n",
    "![Alt text](./img/prob50205.png)\n",
    "\n",
    "At (0,1): No feasible descent directions. All feasible directions are ascent directions. This means ${\\bf\n",
    "x}_*=(0,1)^T$ is the minimizer.\n",
    "\n",
    "Applying the KKT conditions at (0,1)\n",
    "\n",
    "* Necessary conditions: $g_2$ and $g_3$ are active $\\Rightarrow$ $\\mu_1$ and $\\mu_4$ equal 0.\n",
    "\n",
    "$$\n",
    "\\begin{equation*}\n",
    "\\begin{aligned}\n",
    "&\\nabla f-{\\mu}^T\\nabla {\\bf g}={\\bf 0}^T \\\\\n",
    "&\\Rightarrow \\left(\\begin{array}{c}\n",
    "2(x_1+1)\\\\2(x_2-2)\\end{array}\\right) + \\left(\\begin{array}{c}\n",
    "-\\mu_3\\\\\\mu_2\\end{array}\\right) =\\left.\\left(\\begin{array}{c}\n",
    "0\\\\0\\end{array}\\right)\\right|_{(x_1,x_2)=(0,1)}\\\\\n",
    "&\\Rightarrow \\left(\\begin{array}{c}\n",
    "2-\\mu_3\\\\-2+\\mu_2)\\end{array}\\right)=\\left(\\begin{array}{c}\n",
    "0\\\\0\\end{array}\\right)\\Rightarrow \\mu_2=2,\\ \\mu_3=2\n",
    "\\end{aligned}\n",
    "\\end{equation*}\n",
    "$$\n",
    "\n",
    "The KKT necessary conditions are satisfied at (0,1).\n",
    "\n",
    "* Sufficient conditions: The Hessian of Lagrangian is \n",
    "\n",
    "$$\n",
    "\\begin{equation*}\n",
    "\\left(\\begin{array}{r r} 2&0\\\\0&2\\end{array}\\right),\n",
    "\\end{equation*}\n",
    "$$\n",
    "\n",
    "which is positive definite everywhere. Therefore, ${\\bf x}_*=(0,1)^T$ is the global minimum verifying the graphical solution.\n",
    "\n",
    "\n",
    "\n",
    "### Problem 2 (10 Points)\n",
    "\n",
    "Graph the problem \n",
    "\n",
    "$$\n",
    "\\begin{aligned}\n",
    "\\min_{x_1,x_2} & \\quad  f=-x_1\\\\\n",
    "{\\text{subject to }} & \\quad g_1=x_2-(1-x_1)^3\\leq 0{\\quad} {\\rm and}{\\quad} x_2\\geq 0.\n",
    "\\end{aligned}\n",
    "$$ \n",
    "\n",
    "Find the solution graphically. Then apply the optimality conditions. Can you find a solution based on the optimality conditions? Why? (From Kuhn and Tucker, 1951.)\n",
    "\n",
    "\n",
    "### Solution\n",
    "\n",
    "![Alt text](./img/prob50401.png)\n",
    "\n",
    "From the graph we find the solution is at $(x_{1*},x_{2*})=(1,0)$.\n",
    "\n",
    "Checking the KKT conditions\n",
    "\n",
    "$$\n",
    "\\begin{aligned}\n",
    "&\\left(\\begin{array}{c}-1\\\\0\\end{array}\\right) + \\mu_1\n",
    "\\left(\\begin{array}{c}3(1-x_1^2)\\\\1\\end{array}\\right) +\n",
    "\\mu_2\\left(\\begin{array}{c}0\\\\-1\\end{array}\\right) =\n",
    "\\left(\\begin{array}{c}0\\\\0\\end{array}\\right)\\\\\n",
    "&\\begin{array}{ll} \\mu_1(x_2-(1-x_1)^3)=0,&\\mu_1\\geq0\\\\\n",
    "-\\mu_2x_2=0,&\\mu_2\\geq0\\end{array}\n",
    "\\end{aligned}\n",
    "$$\n",
    "\n",
    "at $(x_{1*},x_{2*})=(1,0)$,\n",
    "\n",
    "$$\n",
    "\\begin{equation*}\n",
    "\\left(\\begin{array}{c}-1\\\\0\\end{array}\\right) + \\mu_1\n",
    "\\left(\\begin{array}{c}0\\\\1\\end{array}\\right) +\n",
    "\\mu_2\\left(\\begin{array}{c}0\\\\-1\\end{array}\\right) =\n",
    "\\left(\\begin{array}{c}0\\\\0\\end{array}\\right) \\Rightarrow\n",
    "\\begin{array} {l} -1 = 0 \\hbox{ : contradict}\\\\ \\mu_1-\\mu_2=0\\end{array}\n",
    "\\end{equation*}\n",
    "$$\n",
    "\n",
    "Hence, this point is not a KKT point because this is not a regular\n",
    "point.\n",
    "\n",
    "\n",
    "### Problem 3 (30 Points)\n",
    "\n",
    "Find a local solution to the problem \n",
    "\n",
    "$$\n",
    "\\begin{aligned}\n",
    "\\max_{x_1,x_2,x_3} & \\quad  f=x_1x_2+x_2x_3+x_1x_3\\\\\n",
    "{\\text{subject to }} & \\quad h=x_1+x_2+x_3-3=0.\n",
    "\\end{aligned}\n",
    "$$ \n",
    "\n",
    "Use two methods: reduced gradient and Lagrange multipliers.\n",
    "\n",
    "\n",
    "### Solution\n",
    "\n",
    "* Reduced gradient\n",
    "\n",
    "Let $d_1=x_1$, $d_2=x_2$ and $s_1=x_3$.\n",
    "\n",
    "$$\n",
    "\\begin{aligned}\n",
    "\\partial z/\\partial{\\bf d} &= (\\partial f/\\partial{\\bf d})\n",
    "- (\\partial f/\\partial{\\bf s})(\\partial{\\bf h}/\\partial{\\bf\n",
    "s})^{-1}(\\partial{\\bf h}/\\partial {\\bf d})\\\\\n",
    "&=\\left(\\begin{array}{c}x_2+x_3\\\\x_1+x_3\\end{array}\\right) -\n",
    "(x_1+x_2)(1)^{-1}\\left(\\begin{array}{c}1\\\\1\\end{array}\\right)\\\\\n",
    "&=\\left(\\begin{array}{c}-x_1+x_3\\\\-x_2+x_3\\end{array}\\right)=\\left(\\begin{array}{c}0\\\\0\\end{array}\\right)\n",
    "\\rightarrow x_1=x_2=x_3\n",
    "\\end{aligned}\n",
    "$$\n",
    "\n",
    "Solving $h=x_1+x_2+x_3-3=3x_1-3=0$, we get\n",
    "$$\n",
    "\\begin{eqnarray*}\n",
    "x_{1*}=x_{2*}=x_{3*}=1 \\hbox{ and } f_*=3\n",
    "\\end{eqnarray*}\n",
    "$$\n",
    "\n",
    "* Lagrangian Method\n",
    "\n",
    "We derive the Lagrangian by first converting the problem to negative-null form.\n",
    "$$\n",
    "\\begin{eqnarray*}\n",
    "L&=& -f+\\lambda h = -x_1x_2-x_2x_3-x_3x_1+\\lambda(x_1+x_2+x_3-3)\\\\\n",
    "\\nabla L&\\Rightarrow&\\left.\\begin{array}{cl}-x_2-x_3+\\lambda &=0\\\\\n",
    "-x_1-x_2+\\lambda &=0\\\\\n",
    "-x_1-x_3+\\lambda &=0\\end{array}\\right\\} \\Rightarrow\n",
    "x_{1*}=x_{2*}=x_{3*}=1,\\ \\lambda =2 \\hbox{ and } f_*=3\n",
    "\\end{eqnarray*}\n",
    "$$\n",
    "Checking the Second order sufficiency\n",
    "$$\n",
    "\\begin{eqnarray*}\n",
    "\\partial{\\bf x}^T L_{\\bf xx} \\partial{\\bf x} = -2(\\partial x_1\\partial\n",
    "x_2+\\partial x_2\\partial x_3+\\partial x_3\\partial x_1)\n",
    "\\end{eqnarray*}\n",
    "$$\n",
    "Since $\\nabla h\\partial{\\bf x} = \\partial x_1+\\partial\n",
    "x_2+\\partial x_3=0$,\n",
    "$$\n",
    "\\begin{eqnarray*}\n",
    "\\partial{\\bf x}^T L_{\\bf xx} \\partial{\\bf x} = 2(\\partial x_1^2+\\partial\n",
    "x_2^2+\\partial x_1\\partial x_2)=((\\partial x_1+\\partial\n",
    "x_2/2)^2+\\frac{4}{3}\\partial x_2^2)\\geq0\n",
    "\\end{eqnarray*}\n",
    "$$\n",
    "Further, for $\\partial{\\bf x}^T L_{\\bf xx} \\partial{\\bf x}$ to be 0, $\\partial x_1$ and $\\partial x_2$ has to be 0, in which case $\\partial x_3$ is also 0, leading to $\\partial x=0$ which is not a perturbation. Therefore, $\\partial{\\bf x}^T L_{\\bf xx} \\partial{\\bf x}>0$ for any non-zero feasible perturbations.\n",
    "\n",
    "This proves that ${\\bf x_*}=(1,1,1)$ is a global maximum to the original problem.\n",
    "\n",
    "\n",
    "### Problem 4 (20 Points)\n",
    "\n",
    "Use reduced gradient to\tfind the value(s) of the parameter $b$ for which the point $x_1=1$, $x_2=2$ is the solution to the problem \n",
    "\n",
    "$$\n",
    "\\begin{aligned}\n",
    "\\max_{x_1,x_2} & \\quad  f=2x_{1} + bx_2\\\\\n",
    "{\\text{subject to }} & \\quad g_1 = x_{1}^{2}+ x_{2}^{2}-5\\leq 0\\\\\n",
    "& \\quad g_2= x_1- x_2-2\\leq 0.\n",
    "\\end{aligned}\n",
    "$$ \n",
    "\n",
    "### Solution\n",
    "\n",
    "Rewrite the problem in the negative null form \n",
    "\n",
    "$$\n",
    "\\begin{equation*}\n",
    "\\begin{aligned}\n",
    "{\\hbox{min}} & \\quad f=-2x_{1} - bx_2\\\\\n",
    "{\\hbox{subject to}} & \\quad g_1 = x_{1}^{2}+ x_{2}^{2}-5\\leq 0\\\\\n",
    "{\\hbox{and}} & \\quad g_2= x_1- x_2-2\\leq 0.\n",
    "\\end{aligned}\n",
    "\\end{equation*}\n",
    "$$\n",
    "\n",
    "At $x_1=1$ and $x_2=2$, $g_1$ is active. Hence, we can consider it\n",
    "as an equality constraint.\n",
    "\n",
    "let $x_1=s$ and $x_2=d$,\n",
    "\n",
    "$$\n",
    "\\begin{equation*}\n",
    "\\begin{aligned}\n",
    "\\partial z/\\partial{\\bf d}|_{(1,2)} &= (\\partial f/\\partial{\\bf d})\n",
    "- (\\partial f/\\partial{\\bf s})(\\partial{\\bf h}/\\partial{\\bf\n",
    "s})^{-1}(\\partial{\\bf h}/\\partial {\\bf d})|_{(1,2)}\\\\\n",
    "&=-b-(-2)(2x_1)^{-1}(2x_2)|_{(1,2)}\\\\\n",
    "&=-b-(-2)(2)^{-1}(4)=0\n",
    "\\end{aligned}\n",
    "\\end{equation*}\n",
    "$$\n",
    "\n",
    "Therefore, $b=4$.\n",
    "\n",
    "Check 2nd-order sufficiency conditions using reduced gradient.\n",
    "$$\n",
    "\\begin{equation*}\n",
    "\\begin{aligned}\n",
    "\\frac{\\partial^2z}{\\partial{\\bf d}^2} &= ({\\bf I},(\\partial{\\bf\n",
    "s}/\\partial{\\bf d})^T) \\left(\\begin{array}{cc}\n",
    "\\frac{\\partial^2f}{\\partial{\\bf d}^2} &\n",
    "\\frac{\\partial^2f}{\\partial\n",
    " {\\bf d} \\partial{\\bf s}}\\\\\n",
    "\\frac{\\partial^2f}{\\partial{\\bf s} \\partial{\\bf d}} &\n",
    "      \\frac{\\partial^2f}{\\partial{\\bf s}^2}\n",
    "\\end{array}\\right)\n",
    " \\left(\\begin{array}{c} {\\rm I}\\\\ \\frac{\\partial{\\bf s}}{\\partial{\\bf d}}\n",
    "\\end{array}\\right) + \\left(\\frac{\\partial f}{\\partial {\\bf s}}\\right)\n",
    "\\left(\\frac{\\partial^2{\\bf s}}{\\partial{\\bf d}^2}\\right)\\\\\n",
    "&=\\left(\\frac{\\partial f}{\\partial {\\bf s}}\\right)\n",
    "\\left(\\frac{\\partial^2{\\bf s}}{\\partial{\\bf d}^2}\\right) \\quad\n",
    "(\\hbox{Since} f_{\\bf xx}={\\bf 0})\\\\\n",
    "&=\\left.- ({\\partial f}/{\\partial {\\bf s}})({\\partial {\\bf\n",
    "h}}/{\\partial {\\bf s}})^{-1}({\\bf I},(\\partial{\\bf s}/\\partial{\\bf\n",
    "d})^T){\\bf\n",
    "h}_{{\\bf xx}}({\\bf I},(\\partial {\\bf s}/\\partial{\\bf d}))^T\\right|_{(1,2)}\\\\\n",
    "&=\\left.- (-2)(2x_2)^{-1}({\\bf I},(2x_1)^{-1}(2x_2)^T)\n",
    "\\left(\\begin{array}{rr} 2 & 0 \\\\ 0 & 2\\end{array}\\right)({\\bf I},(2x_1)^{-1}(2x_2))^T\\right|_{(1,2)}\\\\\n",
    "&=-(-2)(4)^{-1}(2+2(x_2/x_1)^2)|_{(1,2)}\\\\\n",
    "&=5>0\n",
    "\\end{aligned}\n",
    "\\end{equation*}\n",
    "$$\n",
    "Therefore, $b=4$ and $x_1=1$ and $x_2=2$ is a local minimizer.\n",
    "\n",
    "* Alternative Solution\n",
    "\n",
    "Check 2nd-order sufficiency conditions using KKT. The Lagrangian function is\n",
    "$$\n",
    "\\begin{equation}\n",
    "    L(x_1,x_2,\\mu_1,\\mu_2) = -2x_1-4x_2 + \\mu_1(x_1^2+x_2^2-5) + \\mu_2(x_1-x_2-2)\n",
    "\\end{equation}\n",
    "$$\n",
    "Then its gradient and Hessian wrt $\\textbf{x}$ are\n",
    "$$\n",
    "\\begin{equation}\n",
    "    L_x(x_1,x_2,\\mu_1,\\mu_2) = [-2 + 2 \\mu_1 x_1 + \\mu_2, -4 + 2 \\mu_1 x_2 - \\mu_2]^T,\n",
    "\\end{equation}\n",
    "$$\n",
    "and \n",
    "$$\n",
    "\\begin{equation}\n",
    "    L_{xx}(x_1,x_2,\\mu_1,\\mu_2) = [2 \\mu_1, 0; 0, 2 \\mu_1].\n",
    "\\end{equation}\n",
    "$$\n",
    "Since $L_x(x_1,x_2,\\mu_1,\\mu_2)={\\bf 0}$ for $x_1=1$, $x_2=2$ and $\\mu_2=0$ ($g_2$ inactive), we have $\\mu_1 = 1$. Thus $L_{xx}(x_1,x_2,\\mu_1,\\mu_2) = [2, 0; 0, 2]$, p.d. Therefore $x_1=1$ and $x_2=2$ is a local minimizer.\n",
    "\n",
    "\n",
    "\n",
    "### Problem 5 (30 Points)\n",
    "\n",
    "Find the solution for \n",
    "\n",
    "$$\n",
    "\\begin{aligned}\n",
    "\\min_{x_1,x_2,x_3} & \\quad  f=x_{1}^{2}+x_{2}^{2}+x_{3}^{2}\\\\\n",
    "{\\text{subject to }} & \\quad h_1 = x_{1}^{2}/4+x_{2}^{2}/5+x_{3}^{2}/25-1=0\\\\\n",
    "& \\quad h_2 = x_1+x_2-x_3= 0,\n",
    "\\end{aligned}\n",
    "$$ \n",
    "\n",
    "by implementing the generalized reduced gradient algorithm."
   ]
  },
  {
   "cell_type": "code",
   "execution_count": null,
   "id": "representative-replica",
   "metadata": {},
   "outputs": [],
   "source": []
  }
 ],
 "metadata": {
  "kernelspec": {
   "display_name": "Python 3",
   "language": "python",
   "name": "python3"
  },
  "language_info": {
   "codemirror_mode": {
    "name": "ipython",
    "version": 3
   },
   "file_extension": ".py",
   "mimetype": "text/x-python",
   "name": "python",
   "nbconvert_exporter": "python",
   "pygments_lexer": "ipython3",
   "version": "3.7.3"
  },
  "pycharm": {
   "stem_cell": {
    "cell_type": "raw",
    "metadata": {
     "collapsed": false
    },
    "source": []
   }
  }
 },
 "nbformat": 4,
 "nbformat_minor": 5
}
